rename state consistency definitions

viper-total-heaps/Consistency.thy
@@ -4,6 +4,25 @@ begin
 
 section \<open>Definition\<close>
 
+inductive total_heap_consistent_unfold_n_all :: "'a total_context \<Rightarrow> 'a total_state \<Rightarrow> nat \<Rightarrow> bool"
+  for ctxt :: "'a total_context"
+  where
+  Zero: "\<lbrakk>
+    valid_heap_mask (get_mh_total \<phi>)
+  \<rbrakk> \<Longrightarrow>
+    total_heap_consistent_unfold_n_all ctxt \<phi> 0"
+| UnfoldStep: "\<lbrakk>
+    \<And> pred_id vs q \<phi>'. q = get_mp_total \<phi> (pred_id, vs) \<Longrightarrow> q > 0 \<Longrightarrow>
+      unfold_rel ctxt (\<lambda>_. True) pred_id vs q \<phi> \<phi>' \<and> valid_heap_mask (get_mh_total \<phi>') \<and>
+      \<comment> \<open>Do we need \<^term>\<open>valid_heap_mask\<close> above? It should be equivalent without it?
+         Is it easy to prove? Which one is easier to use? Same questions apply to the other definition.\<close>
+      total_heap_consistent_unfold_n_all ctxt \<phi>' n
+  \<rbrakk> \<Longrightarrow>
+    total_heap_consistent_unfold_n_all ctxt \<phi> (Suc n)"
+
+definition total_heap_consistent_all :: "'a total_context \<Rightarrow> 'a total_state \<Rightarrow> bool" where
+  "total_heap_consistent_all ctxt \<phi> \<equiv> \<forall> n. total_heap_consistent_unfold_n_all ctxt \<phi> n"
+
 inductive total_heap_consistent_unfold_n :: "'a total_context \<Rightarrow> 'a total_state \<Rightarrow> nat \<Rightarrow> bool"
   for ctxt :: "'a total_context"
   where
@@ -12,33 +31,14 @@ inductive total_heap_consistent_unfold_n :: "'a total_context \<Rightarrow> 'a t
   \<rbrakk> \<Longrightarrow>
     total_heap_consistent_unfold_n ctxt \<phi> 0"
 | UnfoldStep: "\<lbrakk>
-    \<And> pred_id vs q \<phi>'. q = get_mp_total \<phi> (pred_id, vs) \<Longrightarrow> q > 0 \<Longrightarrow>
+    \<And> pred_id vs q \<phi>'. q \<le> get_mp_total \<phi> (pred_id, vs) \<Longrightarrow> q > 0 \<Longrightarrow>
       unfold_rel ctxt (\<lambda>_. True) pred_id vs q \<phi> \<phi>' \<and> valid_heap_mask (get_mh_total \<phi>') \<and>
-      \<comment> \<open>Do we need \<^term>\<open>valid_heap_mask\<close> above? It should be equivalent without it?
-         Is it easy to prove? Which one is easier to use? Same questions apply to the other definition.\<close>
       total_heap_consistent_unfold_n ctxt \<phi>' n
   \<rbrakk> \<Longrightarrow>
     total_heap_consistent_unfold_n ctxt \<phi> (Suc n)"
 
 definition total_heap_consistent :: "'a total_context \<Rightarrow> 'a total_state \<Rightarrow> bool" where
   "total_heap_consistent ctxt \<phi> \<equiv> \<forall> n. total_heap_consistent_unfold_n ctxt \<phi> n"
-
-inductive total_heap_consistent_amount_unfold_n :: "'a total_context \<Rightarrow> 'a total_state \<Rightarrow> nat \<Rightarrow> bool"
-  for ctxt :: "'a total_context"
-  where
-  Zero: "\<lbrakk>
-    valid_heap_mask (get_mh_total \<phi>)
-  \<rbrakk> \<Longrightarrow>
-    total_heap_consistent_amount_unfold_n ctxt \<phi> 0"
-| UnfoldStep: "\<lbrakk>
-    \<And> pred_id vs q \<phi>'. q \<le> get_mp_total \<phi> (pred_id, vs) \<Longrightarrow> q > 0 \<Longrightarrow>
-      unfold_rel ctxt (\<lambda>_. True) pred_id vs q \<phi> \<phi>' \<and> valid_heap_mask (get_mh_total \<phi>') \<and>
-      total_heap_consistent_unfold_n ctxt \<phi>' n
-  \<rbrakk> \<Longrightarrow>
-    total_heap_consistent_amount_unfold_n ctxt \<phi> (Suc n)"
-
-definition total_heap_consistent_amount :: "'a total_context \<Rightarrow> 'a total_state \<Rightarrow> bool" where
-  "total_heap_consistent_amount ctxt \<phi> \<equiv> \<forall> n. total_heap_consistent_amount_unfold_n ctxt \<phi> n"
 
 
 section \<open>Auxiliary Lemmas\<close>
@@ -56,21 +56,17 @@ lemma iff_intro:
 
 section \<open>Theorems\<close>
 
-lemma "total_heap_consistent ctxt \<phi> \<longleftrightarrow> total_heap_consistent_amount ctxt \<phi>" (is "?LHS \<longleftrightarrow> ?RHS")
+lemma "total_heap_consistent_all ctxt \<phi> \<longleftrightarrow> total_heap_consistent ctxt \<phi>" (is "?LHS \<longleftrightarrow> ?RHS")
 proof (rule iff_intro)
   show "?LHS \<longrightarrow> ?RHS"
-  proof (simp add: total_heap_consistent_def total_heap_consistent_amount_def, rule forall_implies)
-    fix n show "total_heap_consistent_unfold_n ctxt \<phi> n \<Longrightarrow> total_heap_consistent_amount_unfold_n ctxt \<phi> n"
+  proof (simp add: total_heap_consistent_all_def total_heap_consistent_def, rule forall_implies)
+    fix n show "total_heap_consistent_unfold_n_all ctxt \<phi> n \<Longrightarrow> total_heap_consistent_unfold_n ctxt \<phi> n"
     proof (induct n arbitrary: \<phi>)
       case 0 then show ?case
-        using total_heap_consistent_amount_unfold_n.Zero total_heap_consistent_unfold_n.cases by blast
+        using total_heap_consistent_unfold_n.Zero total_heap_consistent_unfold_n_all.cases by blast
     next
       case IH: (Suc n)
       show ?case sorry
-      (* proof (simp add: total_heap_consistent_amount_unfold_n.simps, standard,
-             (rule allI)+, standard, standard)
-        fix pred_id vs q
-        assume "q \<le> get_mp_total \<phi> (pred_id, vs)" and "q > 0" *)
     qed
   qed
 next
